src/typechecker/FStarC.TypeChecker.Util.fsti
@@ -56,8 +56,8 @@ val lcomp_univ_opt: lcomp -> (option universe & guard_t)
 val is_pure_effect: env -> lident -> bool
 val is_pure_or_ghost_effect: env -> lident -> bool
 val should_not_inline_lc: lcomp -> bool
-val bind: Range.range -> env -> option term -> lcomp -> lcomp_with_binder -> lcomp
-val maybe_return_e2_and_bind: Range.range -> env -> option term -> lcomp -> e2:term -> lcomp_with_binder -> lcomp
+val bind: Range.range -> is_let_binding:bool -> env -> option term -> lcomp -> lcomp_with_binder -> lcomp
+val maybe_return_e2_and_bind: Range.range -> is_let_binding:bool -> env -> option term -> lcomp -> e2:term -> lcomp_with_binder -> lcomp
 
 (*
  * When typechecking a match term, typechecking each branch returns
